src/Crypto/AESEncryption.dfy
@@ -2,6 +2,7 @@ include "../StandardLibrary/StandardLibrary.dfy"
 include "Cipher.dfy"
 
 module {:extern "AESEncryption"} AESEncryption {
+    //TODO This code has yet to be reviewed. See issue #36
     import C = Cipher
     import opened StandardLibrary
     import opened UInt = StandardLibrary.UInt
@@ -22,13 +23,17 @@ module {:extern "AESEncryption"} AESEncryption {
             k := C.GenKey(cipher);
         }
 
-        static function method {:extern "aes_decrypt"} aes_decrypt(cipher : C.CipherParams, taglen : uint8, key : seq<uint8>, ctxt : seq<uint8>, iv : seq<uint8>, aad : seq<uint8>) : Result<seq<uint8>>
+        static function method {:extern "aes_decrypt"} aes_decrypt(cipher: C.CipherParams,
+                                                      key: seq<uint8>,
+                                                      ctxt: seq<uint8>,
+                                                      iv: seq<uint8>,
+                                                      aad: seq<uint8>): Result<seq<uint8>>
             requires |key| == C.KeyLengthOfCipher(cipher) as int
 
-        static function method AESDecrypt(cipher : C.CipherParams, k : seq<uint8>, md : seq<uint8>, c : seq<uint8>) : Result<seq<uint8>>
+        static function method AESDecrypt(cipher: C.CipherParams, k: seq<uint8>, md: seq<uint8>, c: seq<uint8>): Result<seq<uint8>>
             requires AESWfKey(cipher, k)
             requires AESWfCtx(cipher, c) {
-            match aes_decrypt(cipher, cipher.tagLen, k, c[cipher.ivLen ..], c[0 .. cipher.ivLen], md)
+            match aes_decrypt(cipher, k, c[cipher.ivLen ..], c[0 .. cipher.ivLen], md)
                 case Failure(e) => Failure(e)
                 case Success(m) => Success(m)
             }
@@ -43,7 +48,7 @@ module {:extern "AESEncryption"} AESEncryption {
             requires |iv| == cipher.ivLen as int
             requires |key| == C.KeyLengthOfCipher(cipher) as int
             ensures ctx.Success? ==> |ctx.value| > (cipher.tagLen) as int
-            ensures ctx.Success? ==> aes_decrypt(cipher, cipher.tagLen, key, ctx.value, iv, aad) == Success((msg))
+            ensures ctx.Success? ==> aes_decrypt(cipher, key, ctx.value, iv, aad) == Success((msg))
 
         static method AESEncrypt(cipher : C.CipherParams, k : seq<uint8>, msg : seq<uint8>, md : seq<uint8>) returns (c : Result<seq<uint8>>)
             requires AESWfKey(cipher, k)
