src/StandardLibrary/StandardLibrary.dfy
@@ -48,6 +48,10 @@ module {:extern "STL"} StandardLibrary {
     }
   }
 
+  predicate StringIs8Bit(s: string) {
+    forall i :: i in s ==> i < 256 as char
+  }
+
   function Fill<T>(value: T, n: nat): seq<T>
     ensures |Fill(value, n)| == n
     ensures forall i :: 0 <= i < n ==> Fill(value, n)[i] == value
@@ -63,13 +67,13 @@ module {:extern "STL"} StandardLibrary {
     a := new T[|s|](i requires 0 <= i < |s| => s[i]);
   }
 
-  function method byteseq_of_string (s : string) : (s' : seq<uint8>)
+  function method StringToByteSeq (s : string) : (s' : seq<uint8>)
     requires forall i :: i in s ==> i < 256 as char
-    ensures |s| == |s'|
+    ensures |s| == |s'| 
   {
       if s == [] then [] else  (
         assert (forall i :: i in s[1..] ==> i in s);
-        [(s[0] as int % 256) as uint8] + byteseq_of_string(s[1..]))
+        [(s[0] as int % 256) as uint8] + StringToByteSeq(s[1..]))
   }
 
   function method byteseq_of_string_lossy (s : string) : (s' : seq<uint8>)
@@ -80,16 +84,16 @@ module {:extern "STL"} StandardLibrary {
         [(s[0] as int % 256) as uint8] + byteseq_of_string_lossy(s[1..]))
   }
 
-  function method string_of_byteseq (s : seq<uint8>) : (s' : string)
-    ensures |s| == |s'|
+  function method ByteSeqToString (s : seq<uint8>) : (s' : string)
+    ensures |s| == |s'| 
     ensures forall i :: i in s' ==> i < 256 as char
   {
-      if s == [] then [] else [(s[0] as char)] + string_of_byteseq(s[1..])
+      if s == [] then [] else [(s[0] as char)] + ByteSeqToString(s[1..])
   }
 
-  lemma string_byteseqK (s : string)
-    requires forall i :: i in s ==> i < 256 as char
-    ensures string_of_byteseq(byteseq_of_string(s)) == s {
+  lemma StringByteSeqCorrect(s: string)
+    requires StringIs8Bit(s)
+    ensures ByteSeqToString(StringToByteSeq(s)) == s {
       if s == [] {
 
       }
@@ -100,8 +104,8 @@ module {:extern "STL"} StandardLibrary {
       }
     }
 
-  lemma byteseq_stringK (s : seq<uint8>)
-    ensures byteseq_of_string(string_of_byteseq(s)) == s {
+  lemma ByteSeqStringCorrect(s: seq<uint8>)
+    ensures StringToByteSeq(ByteSeqToString(s)) == s {
 
     }
 
